\section{Binomische Formeln LÃ¶sung}
Autor: Katja Matthes

\subsubsection{Aufgabe 1} 
\begin{enumerate}
%\begin{multicols}{2}
	\item \quad $ (4x + 3y^3)^2=16x^2 + 24xy^3 + 9y^6 $					% 9
	\item \quad $ -(x^4-2)^2=-x^8 + 4x^4 - 4 $								%10
	\item \quad $ (x^2-x^3)(x^2+x^3) =x^4 - x^6 $											%11
	\item \quad $ (3x^2+2t)^2 =9x^4 + 12x^2t + 4t^2 $					%12
	\item \quad $ -\frac{1}{2}(x^2-4)^2 =-\frac{1}{2}x^4 + 4x^2 - 8 $		%13
	\item \quad $ \left(-\frac{1}{2}(x^2-4)\right)^2 =\frac{1}{4}x^4 -2x^2 + 4 $			%14
	\item \quad $ x^2y^2(x^4+2x^2y+y^2) =(x^3y+xy^2)^2 $									%15
%	\end{multicols} 
\end{enumerate}

\subsubsection{Aufgabe 2} 
\begin{enumerate}
%\begin{multicols}{2}
	\item \quad $ (x-3)^n \cdot (x+3)^n =(x^2 - 9)^n $										% 1
	\item \quad $ \frac{(a^2-b^2)^3}{(a-b)^3}=(a+b)^3 $												% 2
	\item \quad $ \frac{(4-x^2)^n}{(2-x)^n}=(2+x)^n $												% 3
	\item \quad $ \frac{(c-1)^{n-1}}{(c^2-1)^{n-1}} =\frac{1}{(c+1)^{n-1}} $					% 4
	\item \quad $ \frac{(a^{2n}-b^{2n})^2}{(a^n-b^n)^2} =(a^n+b^n)^2 $										% 5
	\item \quad $ (a^3 - ab^2)(a+b)^2=a(a-b)(a+b)^3 $									% 6
	\item \quad $ \frac{[(x-y)^2]^k}{(x^2-y^2)^k} =\left(\frac{x-y}{x+y}\right)^k $% 7
	\item \quad $ (a+b)^4(a-b)^4(a^2-b^2)^5=(a^2 - b^2)^9 $									% 8
%	\end{multicols} 
\end{enumerate}

\subsubsection{Aufgabe 3}
\begin{enumerate}
%\begin{multicols}{2}
	\item \quad $ (3x-6)\left(\frac{1}{4}x^2 - x + 1\right)=\frac{3(x-2)^3}{4} $			% 1
	\item \quad $ a^2 - 2a^3 + a^4=a^2(1-a)^2 $							% 2
	\item \quad $  3a^3 - 12a^9=3a^2(1-2a^3)(1+2a^3)=3a^2(1-4a^6) $		% 3
	\item \quad $ x^4 - a^2 =(x^2-a)(x^2+a) $					% 4
	\item \quad $ 3-x^2 =(\sqrt{3}-x)(\sqrt{3}+x) $% 5
	\item \quad $ x^{2n} + 4x^n + 4 =(x^n + 2)^2 $							% 6
	\item \quad $ x^{n+2} -6x^{n+1} + 9x^n =x^n(x-3)^2 $							% 7
	\item \quad $ e^{2x}-1 =(e^x-1)(e^x+1) $					% 8
	\item \quad $ x^2e^x + 2xe^x +e^x =e^x(x+1)^2 $							% 9
%	\end{multicols} 
\end{enumerate}

\subsubsection{Aufgabe 4} 
\begin{enumerate}
%\begin{multicols}{2}
	\item \quad $ \frac{a^3+2a^2b+ab^2}{(a+b)^2} =a $															% 1
	\item \quad $ \frac{a^4-a^2b^2}{ab-a^2}=-a(a+b) $												% 2
	\item \quad $ \frac{t^3+6t^2+9t}{t^2-9} =\frac{t(t+3)}{t-3} $						% 3
	\item \quad $ \frac{x^{2n}-10x^n+25}{x^{2n}-25}=\frac{x^n-5}{x^n+5} $						% 4
	\item \quad $ \frac{x^6-t^2}{x^4+tx} =\frac{x^3-t}{x} $								% 5
	\item \quad $ \frac{x^{n+3}-x^{n+1}}{x^{n+1}+x^n}=x(x-1) $												% 6
	\item \quad $ \frac{(x^2+8xy+16y^2)}{(2x-3y)^{-2}} : \frac{x^2-16y^2}{2x-3y}=\frac{(x+4y)(2x-3y)^3}{x-4y} $	% 7
	\item \quad $ \frac{4t^2-4}{t^2+2t+1} =\frac{4(t-1)}{t+1} $						% 8
	\item \quad $ \frac{x^{n-1}-x^n}{x^n-x^{n+2}}=\frac{1}{x(1+x)} $							% 9
	\item \quad $ \frac{2(a^2+b^2)^2}{a^5-ab^4}=\frac{2(a^2+b^2)}{a(a^2-b^2)} $	%10
	\item \quad $ \frac{x^4-x^3}{x^4-x^2} =\frac{x}{x+1} $									%11
	\item \quad $ \frac{x^3y-xy^5}{x^3y^2-x^2y^4}=\frac{x+y^2}{xy} $							%12
	\item \quad $ \frac{am-an+bm-bn}{a^2-b^2} =\frac{m-n}{a-b} $								%13
	%\end{multicols} 
\end{enumerate}

\subsubsection{Aufgabe 5} 
\begin{enumerate}
%\begin{multicols}{2}
	\item \quad $ (e^x+e^{-x})^2 =e^{2x}+e^{-2x}+2 $	% 1
	\item \quad $ (a^2-a^{-2})^2 =a^4 - 2 +a^{-4} $		% 2
	\item \quad $ (x^{-2}-3x)(x^{-2}+3x) =x^{-4}-9x^2 $				% 3
	\item \quad $ (2^{-x}+2^x)(2^{-x}-2^x) =2^{-2x}-2^{2x} $		% 4
%	\end{multicols} 
\end{enumerate}

\subsubsection{Aufgabe 6} 
\begin{enumerate}
%\begin{multicols}{2}
	\item \quad $\frac{e^{2x}-e^{-2x}}{e^x-e^{-x}} = e^x + e^{-x} $	% 1
	\item \quad $\left(\frac{x-y}{a-b}\right)^5 \cdot \left(\frac{x-y}{5}\right)^{-2} \cdot \frac{(a-b)^2}{(x^2-y^2)}=\frac{25(x-y)^2}{(x+y)(a-b)^3} $									% 2
	%\end{multicols} 
\end{enumerate}
\pagebreak