\section{Bruchrechnung LÃ¶sung}
Autor: Katja Matthes
\subsubsection{Aufgabe 1}
\begin{enumerate}
\begin{multicols}{3}
	\item \quad $ \frac{20}{6} = \frac{10}{3} $
	\item \quad $ \frac{92}{4} = 23 $
	\item \quad $ \frac{86}{12} = \frac{43}{6} $
	\item \quad $ \frac{112}{49} = \frac{16}{7} $
	\item \quad $ \frac{360}{25} = \frac{72}{5} $
	\item \quad $ \frac{420}{40} = \frac{21}{2} $
	\item \quad $ \frac{1716}{308}= \frac{39}{7} $
\end{multicols} 
\end{enumerate}

\subsubsection{Aufgabe 2}
\begin{enumerate}
\begin{multicols}{2}
	\item \quad $ \frac{3}{7} \cdot \frac{5}{9} \cdot \frac{28}{45} \cdot \frac{3}{8} = \frac{1}{18} $
  \item \quad $ \frac{56}{65} \cdot 12 \cdot \frac{5}{7} \cdot \frac{13}{16} = 6 $
	\item \quad $ \frac{98}{99} \cdot \frac{13}{14} \cdot \frac{11}{7} \cdot \frac{5}{26} = \frac{5}{18} $
	\item \quad $ \frac{63}{8} \cdot \frac{5}{18} \cdot \frac{32}{33} \cdot \frac{11}{14} = \frac{5}{3} $
	\item \quad $ 1 : \left( \frac{2}{9} + \frac{1}{7} \right) = \frac{63}{23} $
	\item \quad $ \left( \frac{3}{5} - \frac{1}{4} \right) : \frac{3}{4} = \frac{7}{15} $
	\item \quad $ \frac{5}{8} \cdot \left( \frac{1}{6} + \frac{13}{15} \right) = \frac{31}{48} $
	\item \quad $ \left( \frac{9}{11} - \frac{5}{8} \right) \cdot \frac{4}{17} = \frac{1}{22} $
\end{multicols} 
\end{enumerate}
	
\subsubsection{Aufgabe 3}
\begin{enumerate}
\begin{multicols}{3}
	\item \quad $ \frac{\frac{8}{9}}{\frac{16}{27}} = \frac{3}{2} $
	\item \quad $ \frac{\frac{1}{5}}{\frac{9}{10}} = \frac{2}{9} $
	\item \quad $ \frac{2\frac{1}{3}}{1\frac{1}{6}} = 2 $
	\item \quad $ \frac{\frac{5}{8}}{\frac{1}{4}} = \frac{5}{2} $
	\item \quad $ \frac{2\frac{2}{7}}{1\frac{1}{3}} = \frac{12}{7} $
	\item \quad $ \frac{5\frac{1}{2}}{\frac{11}{12}} = 6 $
	\item \quad $ \frac{6\frac{1}{4}}{\frac{15}{16}} = \frac{20}{3} $
	\item \quad $ \frac{\frac{99}{100}}{\frac{9}{10}} = \frac{11}{10} $
\end{multicols} 
\end{enumerate}

\subsubsection{Aufgabe 4}
\begin{enumerate}
%\begin{multicols}{2}
	\item \quad $ \frac{5}{6} \cdot \frac{2}{3} - \frac{2}{9} + \frac{3}{4} \cdot 1\frac{7}{9} = \frac{5}{3} $
	\item \quad $ 5\frac{1}{2} - \frac{3}{7} : \frac{8}{21} + 1\frac{9}{16} : 3\frac{3}{4} = \frac{115}{24} $
	\item \quad $ 1\frac{3}{5} : \frac{4}{15} + \frac{11}{12} - 5\frac{2}{3} + \frac{1}{8} \cdot 4 = \frac{7}{4} $
	\item \quad $ 3\frac{5}{12} - 2\frac{5}{6} + 1\frac{1}{3} : \frac{4}{9} - 2\frac{1}{6} \cdot \frac{1}{2} = \frac{5}{2} $
%\end{multicols} 
\end{enumerate}

\subsubsection{Aufgabe 5}
\begin{enumerate}
\begin{multicols}{2}
	\item \quad $ \left(\frac{2}{3} - \frac{1}{6}\right) \cdot \left(\frac{9}{11} - \frac{3}{7}\right) = \frac{15}{77} $
	\item \quad $ \left(\frac{1}{8} + \frac{7}{12}\right) : \left(5 - \frac{3}{4}\right) = \frac{1}{6} $
	\item \quad $ \frac{4}{7} \cdot \left(\left(1\frac{1}{2} - \frac{5}{9}\right) : 4\frac{1}{4}\right) = \frac{8}{63} $
	\item \quad $ \frac{4}{5} : \left[\left(\frac{5}{8} - \frac{1}{3}\right) \cdot 12\right] = \frac{8}{35} $
	\item \quad $ \frac{3}{4} \cdot \left(2\frac{1}{2} : 1\frac{1}{4}\right) = \frac{3}{2} $
\end{multicols} 
\end{enumerate}

\subsubsection{Aufgabe 6}
\begin{enumerate}
\begin{multicols}{2}
	\item \quad $ 1\frac{1}{2} \cdot 2\frac{1}{4} + \frac{5}{8} = 4 $
	\item \quad $ 2\frac{1}{2} + 1\frac{1}{4} \cdot 1\frac{3}{5} = \frac{9}{2} $
	\item \quad $ 1\frac{1}{2} \cdot 1\frac{1}{3} - 1\frac{1}{3} \cdot 1\frac{1}{4} = \frac{1}{3} $
	\item \quad $ 5\frac{1}{2} \cdot 3 - 3\frac{1}{3} \cdot 4 = \frac{19}{6} $
	\item \quad $ \frac{2}{3} \cdot 5 - 4 \cdot \frac{1}{3} = 2 $
	\item \quad $ 6 \cdot 2\frac{1}{3} - 1\frac{1}{4} \cdot 8 = 4 $
	\item \quad $ 6 \cdot \frac{4}{7} - 2 \cdot \frac{1}{9} = \frac{202}{63} $
	\item \quad $ 3\frac{3}{4} \cdot 2 - 1\frac{2}{7} \cdot 3 = \frac{51}{14} $
	\item \quad $ 2\frac{3}{4} : 2 + \frac{5}{8} = 2 $
	\item \quad $ \frac{4}{5} : 2 - \frac{2}{5} : 3\frac{1}{3} = \frac{7}{25} $
	\item \quad $ 3 : 5\frac{1}{2} - 2 : 3\frac{2}{3} = 0 $
	\item \quad $ 4 : 9 + \frac{1}{2} : \frac{9}{10} = 1 $
	\item \quad $ 4 \cdot \frac{2}{3} - 4 : 6 = 2 $
	\item \quad $ \frac{4}{5} : 3 + 2 : 5 = \frac{2}{3} $
	\item \quad $ 4 : \frac{3}{8} - \frac{5}{3} : 10 = \frac{21}{2} $
	\item \quad $ 8 : 3 - \frac{3}{4} \cdot 2 = \frac{7}{6} $
\end{multicols} 
\end{enumerate}
\newpage
\subsubsection{Aufgabe 7}
\begin{enumerate}
\begin{multicols}{2}
	\item \quad $ \frac{\frac{3}{8} \cdot \frac{2}{7}}{\frac{5}{14}} = \frac{3}{10} $
	\item \quad $ \frac{1\frac{3}{4} + \frac{5}{6}}{\frac{1}{4}} = \frac{31}{3} $
	\item \quad $ \frac{\frac{8}{9}}{3\frac{1}{3} + \frac{1}{6}} = \frac{16}{63} $
	\item \quad $ \frac{\left(\frac{3}{5} - \frac{5}{10}\right) : \frac{2}{5}}{\frac{1}{4} + \frac{1}{2}} = \frac{1}{3} $
	\item \quad $ \frac{\frac{1}{8} : \left(\frac{1}{32} + \frac{3}{4}\right)}{\left(\frac{1}{5} - \frac{2}{25}\right) \cdot \frac{1}{3}} = 4 $
	\item \quad $ \frac{4 + \left(\frac{1}{3} \cdot \left(2\frac{3}{4} - 1\frac{3}{8}\right)\right)}{\left(2\frac{1}{3} : \frac{7}{9}\right) \cdot \left(\left(\frac{1}{4} + 2\frac{5}{8}\right) - 2\right)} = \frac{107}{63} $
	\item \quad $ \frac{\left(\frac{4}{7} + 2\frac{1}{2}\right) \cdot \frac{1}{3} + 1}{\frac{2}{5} \cdot \left(1\frac{3}{4} - \frac{5}{6}\right)} = \frac{425}{77}$
\end{multicols} 
\end{enumerate}
