\section{Potenzen LÃ¶sung}
Autor: Katja Matthes

\subsubsection{Aufgabe 1}
\begin{enumerate}
%\begin{multicols}{2}
	\item \quad $ 3x^4 - x^4 - x^3(x + 2) = x^4 - 2x^3 $								% 1
	\item \quad $ -12a^2 + 3a(a + 1) = -9a^2 + 3a $								% 2
	\item \quad $ ax^n + 4x^n = (a + 4)x^n $								% 3
	\item \quad $ (1-t)^2 - \frac{1}{2}(1-t)^2 = \frac{1}{2}(1 - t)^2 $			% 4
	\item \quad $ a(x+t)^k - b(x+t)^k = (a-b)(x+t)^k $							% 5
	\item \quad $ tx^3 - 3x^2 + 2tx^3 - 4x^2 = 3tx^3 - 7x^2 $							% 6
	\item \quad $ t^3 \cdot t^4 - t^5(t^2+1) = -t^5 $											% 7
	\item \quad $ x^2 \cdot x^3 \cdot x^4 = x^9 $												% 8
	\item \quad $ 3a^k \cdot a^{k-1} \cdot a = 3a^{2k} $										% 9	
	\item \quad $ b^n \cdot b^{2n+1} = b^{3n+1} $									%10
	\item \quad $ (x+1)^{n-1} \cdot (x+1)^{n+1} = (x+1)^{2n} $								%11
	\item \quad $ \left(\frac{x}{3}\right)^4 \cdot \left(\frac{x}{3}\right)^2 = \left(\frac{x}{3}\right)^6 $%12
	\item \quad $ t^2 \cdot x^2 \cdot t^n \cdot x^{n-1} = t^{2+n} x^{n+1} $						%13
	\item \quad $ a \cdot b^k \cdot a^{2n} \cdot b^{k-3} = a^{2n+1} \cdot b^{2k-3} $		%14
	\item \quad $ (x-2)^n \cdot (x-2)^{1-n} = x-2 $												%15
	\item \quad $ 0,3^6 \cdot \left(\frac{10}{3}\right)^6 = 1 $													%16
	\item \quad $ 2^x \cdot \left(\frac{5}{2}\right)^x \cdot 5 = 5^{x+1} $										%17
	\item \quad $ 2^5 \cdot \left(\frac{1}{2}\right)^4 = 2 $													%18	
	\item \quad $ \left(\frac{x}{4}\right)^4 \cdot 4^6 = 4^2x^4 $										%19
	\item \quad $ 2^n \cdot \left(\frac{x}{2}\right)^n \cdot x = x^{n+1} $										%20
	\item \quad $ 9 \cdot 3^{n+1} = 3^{n+3} $										%21
	\item \quad $ (a-b)^9 \cdot (a-b) = (a-b)^{10} $								%22
	\item \quad $ \left(\frac{a-b}{c}\right)^{2k} \cdot \left(\frac{c}{a-b}\right)^{2k} = 1 $													%23	
%\end{multicols} 
\end{enumerate}

\subsubsection{Aufgabe 2}
\begin{enumerate}
\begin{multicols}{2}
	\item \quad $ \frac{a^6}{a^3} = a^3 $																					% 1
	\item \quad $ \frac{x^{2n+1}}{x^n} = x^{n+1} $																			% 2
	\item \quad $ \frac{15e^{x+1}}{5e^x} = 3e $																					% 3
	\item \quad $ \frac{x^4}{x^7} = x^{-3} $																			% 4
	\item \quad $ \frac{2a^{1-2n}}{4a^{n+1}} = \frac{1}{2}a^{-3n} $													% 5
	\item \quad $ \frac{a^4b^{4n+3}}{a^nb^{2n-1}} = a^{4-n}b^{2n+4} $																	% 6
	\item \quad $ \frac{81}{3^{x+3}} = 3^{1-x} $																			% 7
	\item \quad $ \frac{(a-b)^3}{(a-b)^{n-1}} = (a-b)^{4-n} $																	% 8
	\item \quad $ \frac{(ab)^3}{x^2y} \cdot \frac{(xy)^2}{a^4b^2} = \frac{by}{a} $																% 9
	\item \quad $ \frac{a^{n+1}}{a^n} = a $																						%10
	\item \quad $ \frac{10^3}{2^3}=5^3 $																					%11
	\item \quad $ \frac{2,5^4}{0,5^4}=5^4 $																					%12
	\item \quad $ \frac{(10ab)^k}{(4b)^k}=\left(\frac{5}{2}a\right)^k $									%13
	\item \quad $ \left(\frac{a}{b}\right)^n \cdot \frac{a}{b}=\left(\frac{a}{b}\right)^{n+1} $							%16
	\item \quad $ \left(\frac{-1}{a-b}\right)^3=-(a-b)^{-3} $																		%17
	\item \quad $ \left(\frac{x}{2}\right)^3 : \left(\frac{x}{3}\right)=\frac{3}{8}x^2 $															%18
	\item \quad $ (-5^2)^3=-5^6 $																				%19
	\item \quad $ 3(c^4)^3 - 6c^{12}=-3c^{12} $																		%20		
	\item \quad $ (3b^2c^{n-1})^4=81b^8c^{4n-4} $																%21
	\item \quad $ \left(\frac{7a^2}{49b^3}\right)^2=\frac{a^4}{49b^6} $														%22
	\item \quad $ \left(\frac{-1}{c^3}\right)^{2n}=\frac{1}{c^{6n}} $														%23
	\item \quad $ (3b^{n+1} \cdot c^{n-1})^2=9b^{2n+2}c^{2n-2} $														%24	
	\item \quad $ (x^2y^3z^2)^5=x^{10}y^{15}z^{10} $													%25	
	\item \quad $ (0,5e^{x+2})^2=0,25e^{2x+4} $																%26
	\item \quad $ \left(\frac{2}{x^2}\right)^5 - \left(\frac{3}{x^5}\right)^2=\frac{23}{x^{10}} $														%27
	\item \quad $ \left[\left(-\frac{3}{t}\right)^3\right]^4 \cdot \frac{t^9}{81}=\frac{3^8}{t^3} $															%28
	\item \quad $ \frac{(ab)^2}{x^3y} \cdot \frac{x^5y^2}{a^2b}=bx^2y $																				%29
	\item \quad $ (\frac{(4-12x)^3}{64}=1-3x)^3 $																		%30
	\item \quad $ \frac{(2x-4)^5}{(2-x)^3}=-32(2-x)^2 $																	%31
	\item \quad $ \frac{(4ab)^4}{(6a^2)^4} \cdot \frac{5}{b^4}=\frac{80}{81}a^{-4} $													%32
	\item \quad $ (a-b^2) \cdot (a-b^2)^n=(a-b^2)^{n+1} $																%33
		\end{multicols} 
\end{enumerate}


\subsubsection{Aufgabe 3}
\begin{enumerate}
%\begin{multicols}{2}
	\item \quad $ \left(\frac{1}{2}x^2\right)^5 + \frac{1}{8}(x^2)^5 + (2x^5)^2=\frac{133}{32}x^{10} $												%34	
	\item \quad $ \frac{1}{4} \cdot 2^4(2^2)^3=2^8 $																					%35
	\item \quad $ (3^{n+1})^2=3^{2n+2} $																		%36
	\item \quad $ (3x^2 - 5x)(1-x^3) + (x^2 + 3x^4)x^3=3x^7 - 2x^5 + 5x^4 + 3x^2 - 5x $							%37	
	\item \quad $ a^{2r}b^r(a^{2r} - a^rb^{r+1} + b^{2r+2})=a^{4r}b^r - a^{3r}b^{2r+1} + a^{2r}b^{3r+2} $	%38
%	\end{multicols} 
\end{enumerate}

\subsubsection{Aufgabe 4}
\begin{enumerate}
\begin{multicols}{2}
	\item \quad $ -3x^3 \cdot x^2 + 5x \cdot x^4=2x^5 $																				%39
	\item \quad $ 4t^{n-4}t^3-t \cdot t^{n-2}=3t^{n-1} $																		%40
	\item \quad $ 2x^5y^3y - 4x^3y^2x^2y^2=-2x^5y^4 $																		%41
	\item \quad $ \frac{4x^5 + 6x^4 -12x^2}{2x^2}=2x^3 + 3x^2 - 6 $															%42
	\item \quad $ (9 \cdot 3^n - 3^{n+1}) : 3^{n-1}=18 $																					%43
	\item \quad $ (2x+6)^2+(x+3)^2=5(x+3)^2 $																		%44
	\item \quad $ \frac{5a-20}{4a-16}=\frac{5}{4} $																	%45
	\item \quad $ (3t^2 - 3t^3)^2=9t^4(1-t)^2 $																	%46
	\end{multicols} 
\end{enumerate}

\subsubsection{Aufgabe 5}
\begin{enumerate}
\begin{multicols}{2}
	\item \quad $ 3a^2 + 6a^3=3a^2(1+2a) $					% 1
	\item \quad $ \frac{1}{2}e^x - \frac{1}{4}e^{x+1}=\frac{1}{4}e^x(2-e) $	% 2
	\item \quad $ a^{5b} + 3a^b=a^b(a^{4b}+3) $				% 3
	\item \quad $ 2^x + 2^{x+1}=3 \cdot 2^x $					% 4
	\item \quad $ x^4+2x^3=x^3(x+2) $						% 5
	\item \quad $ x^{n+3} - 4x^{n+2}=x^{n+2}(x-4) $				% 6
	\item \quad $ -6t^{n+2}+18t^{2-n}=6t^2(-t^n+3t^{-n}) $	% 7
	\item \quad $ e^x-e^{3x}=e^x(1-e^{2x}) $				% 8
	\end{multicols} 
\end{enumerate}


\subsubsection{Aufgabe 6}
\begin{enumerate}
\begin{multicols}{2}
	\item \quad $ \frac{x^4-x^3}{x^2-x}=x^2 $													% 1
	\item \quad $ \frac{e^{3x}+e^{2x}}{e^{2x}}=e^x + 1 $											% 4
	\item \quad $ \frac{a^7b^3-ab^7}{a^5b-a^2b^4}=\frac{a^6b^2-b^6}{a^4-ab^3} $	% 6
	\item \quad $ \frac{32}{2^{n+5}} + \frac{2^{-n+3}}{8}=\frac{1}{2^{n-1}} $						% 8
\end{multicols} 
\end{enumerate}

\subsubsection{Aufgabe 7}
\begin{enumerate}
%\begin{multicols}{2}
	\item \quad $ y = \frac{1}{4}x^4-2tx^3+\frac{9}{2}t^2x^2 $ mit $ x = 3t \Rightarrow y = \frac{27}{4}t^4 $					% 1
	\item \quad $ y = e^{x^2-t^2}+3e^{5t-(t-x)} $ mit $ x = -t \Rightarrow y = 1 + 3e^{3t} $							% 2
	\item \quad $ y = \frac{3}{2t^2}x^4 - \frac{4}{t}x^3 + 3x^2 - 4 $ mit $ x = \frac{1}{3}t \Rightarrow y = \frac{11}{54}t^2 - 4 $		% 3
	\item \quad $ y = \frac{e^{3tx}+4e^3}{tx-4} $ mit $ x = \frac{1}{t} \Rightarrow y = -\frac{5}{3}e^3 $					% 4
	\item \quad $ y = \frac{tx^3}{2(x+t)^2} $ mit $x = -3t \Rightarrow y = -\frac{27}{8}t^2 $				% 5
%\end{multicols} 
\end{enumerate}

\subsubsection{Aufgabe 8} 
\begin{enumerate}
%\begin{multicols}{2}
	\item \quad $ a^n+a^{4-n}+a^{2n} = a^{2n}(a^{-n}+a^{4-3n}+1) $				% 1
	\item \quad $ a^3 + a^{1-n} + a^{n+4} = a^{n+3}(a^{-n}+a^{-2n-2}+a) $			% 3
	\item \quad $ \frac{3}{2}x^4+\frac{3}{4}x^3+\frac{1}{8}x^2 = \frac{1}{8}x^2(12x^2+6x+1) $			% 4
	\item \quad $ e^{3x}-2e^{-x} = e^{-x}(e^{4x}-2) $								% 5	
	\item \quad $ te^{2x}-2e^{x+1} = e^x(te^x-2e) $										% 6
%	\end{multicols} 
\end{enumerate}

\subsubsection{Aufgabe 9} 
\begin{enumerate}
%\begin{multicols}{2}
	\item \quad $ \frac{1}{4} \cdot 2^{-4} \cdot (2^2)^3 = 1 $									% 1
	\item \quad $ (e^x - e^{-x} + 5)e^x=e^{2x}+5e^x-1 $			% 2
	\item \quad $ 2^x(2^{-1}+2^x)=2^{x-1}+2^{2x} $		% 3	
	\item \quad $ (x^4+x^{-2})(x^3-x^{-3})=x^7-x^{-5} $				% 4
%	\end{multicols} 
\end{enumerate}

\subsubsection{Aufgabe 10}
\begin{enumerate}
\begin{multicols}{2}
	\item \quad $ a^2 \cdot (a^2)^{-2} + 3a \left(\frac{1}{a}\right)^3 =4a^{-2} $														% 1
	\item \quad $ \frac{1}{18} \cdot (3^2)^2 + \frac{1}{2} \cdot 3^3 \cdot \left(\frac{1}{3}\right)^2 =6 $																	% 2
	\item \quad $ (x^2 \cdot x^{-3})^{-2} + \left(\frac{3}{x^2}\right)^{-1} =\frac{4}{3}x^2 $										% 3	
	\item \quad $ a^5 \cdot a^{-2} + 4a^2 \cdot a =5a^3 $															% 4
	\item \quad $ \left(\frac{2}{x}\right)^3 + \left(\frac{1}{x}\right)^3 =\frac{9}{x^3} $											% 6
	\item \quad $ \frac{1}{e^{2x}} + 3(e^{-x})^2 - \left(\frac{2}{e^x}\right)^2 =0 $																	%10
	\item \quad $ e^{-x} \cdot e^{-x+2} \cdot e^{2x-3} =e^{-1} $														%11
	\item \quad $ 6x^3 \cdot x^{-1} - 8x^4 \cdot x^{-2} =-2x^2 $															%13
	\item \quad $ (t^7-t^4) \cdot t^{-3} =t^4-t $															%17
	\end{multicols} 
\end{enumerate}

\subsubsection{Aufgabe 11}
\begin{enumerate}
\begin{multicols}{2}
	\item \quad $ \frac{-2^3 - 2 \cdot 4}{2 \cdot 2^3} =-1 $																% 7
	\item \quad $ \frac{(1-x)^2}{(x-1)} =x-1 $																% 8
	\item \quad $ \frac{e^{3x+1}}{e^{-x+2}} =e^{4x-1} $													% 9
	\item \quad $ \frac{1,5e^{3x} - e^x}{1,5e^{3x}} =1 - \frac{2}{3}e^{-2x} $						%20
	\end{multicols} 
\end{enumerate}

\subsubsection{Aufgabe 12}
\begin{enumerate}
%\begin{multicols}{2}
	\item \quad $ a^4 \cdot a^{-6} - 3a^3 \cdot a^{-5} + a^2 =-2a^{-2} + a^2 $										% 5
	\item \quad $ (a^{n+2} - 4a^n - 2a^{2-n})\cdot \frac{a^{-2}}{2} =\frac{1}{2}a^n - 2a^{n-2} -a^{-n} $	%14
	\item \quad $ 4x^{-4}x^7 - 0,5 x^4x^{-1} + \left(\frac{1}{x^2}\right)^{1,5} =3,5x^3 + \frac{1}{x^3} $						%15
	\item \quad $ \frac{a^{n+1}}{a} + \frac{a^{2n-1}}{a^{n+2}} + (a^{n-1})^2 \cdot a^{2-n} =2a^n + a^{n-3} $										%16
	\item \quad $ \frac{2^{2k}}{8} \cdot 2^{3-k} + 2 \cdot 2^{k-1} =2^{k+1} $														%19
%	\end{multicols} 
\end{enumerate}

\subsubsection{Aufgabe 13}
\begin{enumerate}
	\item \textbf{$ n $ gerade:} \begin{align*} (a-b)^n + (b-a)^n &= (a-b)^n + (-1)^n\cdot(a-b)^n \\
																																&= (a-b)^n + (a-b)^n \\
																																&= 2(a-b)^n \end{align*} \\
				\textbf{$ n $ ungerade:} \begin{align*}  (a-b)^n + (b-a)^n	&= (a-b)^n + (-1)^n\cdot(a-b)^n \\
																																		&= (a-b)^n -(a-b)^n \\
																																		&= 0 \end{align*}							% 1
	\item \textbf{$ n $ gerade:}\begin{align*}  &(x-2)^n + (2x-4)^n - (2-x)^n	\\
																						= &(x-2)^n + (2x-4)^n - (-1)^n\cdot(x-2)^n \\
																						= &(x-2)^n + (2x-4)^n - (x-2)^n \\
																						= &(2x-4)^2 \end{align*}	
				\textbf{$ n $ ungerade:} \begin{align*}	&(x-2)^n + (2x-4)^n - (2-x)^n	\\
																							= &(x-2)^n + 2^n\cdot(x-2)^n - (-1)^n\cdot(x-2)^n \\
																							= &(x-2)^n + 2^n\cdot(x-2)^n + (x-2)^n \\
																							= &2(x-2)^n + 2^n(x-2) \\
																							= &(2+2^n)(x-2)^n \end{align*}% 2
\end{enumerate}
